src/EvalExecs/Constructor.v
@@ -1,42 +1,340 @@
 Require Import UrsusEnvironment.Solidity.current.Environment.
 Require Import UrsusEnvironment.Solidity.current.LocalGenerator.
-
 Require Import UMLang.ExecGenerator.
-Require Import Common.
 
 Require Import EIP20.
+Require Import Common.
+Require Import Templates.Constructor.
 Import EIP20.
 
 
-Definition constructor_exec_sig (_initialAmount :  uint256) 
+Definition constructor_ls_template_exec_sig (_initialAmount :  uint256) 
                                 (_tokenName :  string) 
                                 (_decimalUnits :  uint8) 
                                 (_tokenSymbol :  string) (l : LedgerLRecord rec) :
-                                {t | t = exec_state (Uinterpreter (@constructor rec def _ _ _ _initialAmount _tokenName _decimalUnits _tokenSymbol)) l}.
-  unfold constructor. unfold dynamicAssignL.  
+  {t | t = exec_state (Uinterpreter (@constructor_ls_template rec def _ _ _ _initialAmount _tokenName _decimalUnits _tokenSymbol)) l}.
+  unfold constructor_ls_template. unfold dynamicAssignL. unfold fromUReturnExpression.
   repeat auto_build_P listInfinite.
 Defined.
 
-Definition constructor_exec_let (_initialAmount :  uint256) 
+Definition constructor_ls_template_exec (_initialAmount :  uint256) 
                                 (_tokenName :  string) 
                                 (_decimalUnits :  uint8) 
                                 (_tokenSymbol :  string) (l : LedgerLRecord rec) : LedgerLRecord rec.
-  let_term_of_2_fast @constructor_exec_sig (constructor_exec_sig _initialAmount _tokenName _decimalUnits _tokenSymbol l).
+  let_term_of_2_fast @constructor_ls_template_exec_sig (constructor_ls_template_exec_sig _initialAmount _tokenName _decimalUnits _tokenSymbol l).
 Defined.
 
-Definition constructor_exec (_initialAmount :  uint256) 
+Lemma constructor_ls_template_exec_prf: forall (_initialAmount :  uint256) 
                             (_tokenName :  string) 
                             (_decimalUnits :  uint8) 
-                            (_tokenSymbol :  string) (l : LedgerLRecord rec) : LedgerLRecord rec.
-  flat_term_of_2 @constructor_exec_let (constructor_exec_let _initialAmount _tokenName _decimalUnits _tokenSymbol l).
+                            (_tokenSymbol :  string) (l : LedgerLRecord rec),
+  constructor_ls_template_exec _initialAmount _tokenName _decimalUnits _tokenSymbol l = 
+  exec_state (Uinterpreter (@constructor_ls_template rec def _ _ _ _initialAmount _tokenName _decimalUnits _tokenSymbol)) l.
+Proof.
+  intros.
+  proof_of_2 constructor_ls_template_exec constructor_ls_template_exec_sig 
+             (constructor_ls_template_exec_sig _initialAmount _tokenName _decimalUnits _tokenSymbol l).
+Qed.
+
+Definition constructor_ls_pre_payload_computed' 
+                              (_initialAmount :  uint256) 
+                              (_tokenName :  string) 
+                              (_decimalUnits :  uint8) 
+                              (_tokenSymbol :  string)
+                              (l: LedgerLRecord rec): True.
+    assert (LedgerLRecord rec).
+    remember (constructor_ls_template_exec _initialAmount _tokenName _decimalUnits _tokenSymbol 
+              {$$ l with Ledger_LocalState := default $$}) as exec.
+    destruct_ledger l. 
+
+    time "constructor_ls_template_exec unfold" unfold constructor_ls_template_exec in Heqexec. idtac.
+    
+    time "remember" match goal with
+    | Heql0 : exec = ?L |- _ => match L with
+                                | context [exec_state (Uinterpreter (constructor_ls_payload rec def _ _ _ _ )) ?LL] => 
+                                        remember LL as pre_exec
+                                end
+    end. idtac.
+
+    time "constructor_ls_pre_payload_computed compute" vm_compute in Heqpre_exec. idtac.
+    match goal with
+    | Heql0: pre_exec = ?LL |- _ => transparent_abstract exact_no_check LL using constructor_ls_pre_payload_computed_curried
+    end.
+    exact I.
 Defined.
 
-Definition constructor_prf (_initialAmount :  uint256) 
-                            (_tokenName :  string) 
-                            (_decimalUnits :  uint8) 
-                            (_tokenSymbol :  string) (l : LedgerLRecord rec) :
-  constructor_exec _initialAmount _tokenName _decimalUnits _tokenSymbol l = 
-  exec_state (Uinterpreter (@constructor rec def _ _ _ _initialAmount _tokenName _decimalUnits _tokenSymbol)) l.
-  proof_of_2 constructor_exec constructor_exec_sig (constructor_exec_sig _initialAmount _tokenName _decimalUnits _tokenSymbol l).
+Definition constructor_ls_pre_payload_computed
+                              (_initialAmount :  uint256) 
+                              (_tokenName :  string) 
+                              (_decimalUnits :  uint8) 
+                              (_tokenSymbol :  string)
+                              (l: LedgerLRecord rec): LedgerLRecord rec.     
+remember l as ledger. destruct_ledger l.
+refine (uncurry (f:=_GlobalClass) (constructor_ls_pre_payload_computed_curried _initialAmount _tokenName _decimalUnits _tokenSymbol )
+      (s, (s0, (s1, (s2, (s3, (s4,
+             (c0,
+              (m,
+               (m0,
+                (v0,
+                 (v1,
+                  (v2,
+                   (v3,
+                    (v4,
+                     (v5,
+                      (v6,
+                       (v7, (v8, (v9, (v10, (v11, (v12, (v13, (v14, (v15, (v16, (v17,
+                       l1)))))))))))))))))))))))))))%xprod).
 Defined.
+
+About constructor_ls_payload.
+
+Lemma constructor_ls_template_by_payload: 
+                       forall (_initialAmount_value :  uint256) 
+                              (_tokenName_value :  string) 
+                              (_decimalUnits_value :  uint8) 
+                              (_tokenSymbol_value :  string)
+                              (l: LedgerLRecord rec), 
+  let _initialAmount: ULValue uint256 := local_left_field _ _ _ ("_initialAmount", 1%nat) in
+  let _tokenName: ULValue string := local_left_field _ _ _ ("_tokenName", 1%nat) in
+  let _decimalUnits: ULValue uint8 := local_left_field _ _ _ ("_decimalUnits", 1%nat) in
+  let _tokenSymbol: ULValue string := local_left_field _ _ _ ("_tokenSymbol", 1%nat) in  
+  let pre_exec := constructor_ls_pre_payload_computed _initialAmount_value _tokenName_value _decimalUnits_value _tokenSymbol_value l in  
+
+  constructor_ls_template_exec _initialAmount_value _tokenName_value _decimalUnits_value _tokenSymbol_value 
+                               {$$ l with Ledger_LocalState := default $$} =
+  exec_state (Uinterpreter (@constructor_ls_payload rec def _initialAmount _tokenName _decimalUnits _tokenSymbol)) pre_exec.
+Proof.
+  intros.
+  destruct_ledger l.
+  time "constructor_ls_template_exec unfold" unfold constructor_ls_template_exec. idtac.  
+  time "remember" match goal with
+    | |- context [exec_state (Uinterpreter (constructor_ls_payload rec def ?a1 ?a2 ?a3 ?a4 )) ?LL] => 
+                                        remember LL as pre_exec' 
+  end. idtac.
+
+  time "constructor_ls_pre_payload_computed compute" vm_compute in Heqpre_exec'. idtac.
+
+  time "remember" match goal with
+  | |- context [exec_state (Uinterpreter (constructor_ls_payload rec def ?a1 ?a2 ?a3 ?a4 )) ?LL] => 
+                                      remember a1 as u1
+  end. idtac.
+
+  time "remember" match goal with
+  | |- context [exec_state (Uinterpreter (constructor_ls_payload rec def ?a1 ?a2 ?a3 ?a4 )) ?LL] => 
+                                        remember a2 as u2
+  
+  end. idtac.
+
+  time "remember" match goal with
+  | |- context [exec_state (Uinterpreter (constructor_ls_payload rec def ?a1 ?a2 ?a3 ?a4 )) ?LL] => 
+                                      remember a3 as u3
+  end. idtac.
+
+  time "remember" match goal with
+  | |- context [exec_state (Uinterpreter (constructor_ls_payload rec def ?a1 ?a2 ?a3 ?a4 )) ?LL] => 
+                                      remember a4 as u4
+  end. idtac.  
+
+  
+  assert (u1 = _initialAmount) as H1 by auto.
+  assert (u2 = _tokenName) as H2.
+  subst u2 u1. auto.
+  assert (u3 = _decimalUnits) as H3.
+  subst u3 u2 u1. auto.
+  assert (u4 = _tokenSymbol) as H4.
+  subst u4 u3 u2 u1. auto.
+  
+  rewrite H1, H2, H3, H4. 
+  f_equal. auto.  
+Qed.
+
+
+(* payload *)
+
+Definition constructor_ls_payload_exec_sig (_initialAmount : ULValue uint256) 
+                                           (_tokenName : ULValue string) 
+                                           (_decimalUnits : ULValue uint8) 
+                                           (_tokenSymbol : ULValue string)
+                                           (l : LedgerLRecord rec):
+           {t | t = exec_state (Uinterpreter (@constructor_ls_payload rec def _initialAmount _tokenName _decimalUnits _tokenSymbol)) l}.
+  unfold constructor_ls_payload. 
+  repeat auto_build_P listInfinite.
+Defined.
+
+Definition constructor_ls_payload_exec (_initialAmount : ULValue uint256) 
+                                       (_tokenName : ULValue string) 
+                                       (_decimalUnits : ULValue uint8) 
+                                       (_tokenSymbol : ULValue string)
+                                       (l : LedgerLRecord rec) : LedgerLRecord rec.
+  let_term_of_2_fast @constructor_ls_payload_exec_sig (constructor_ls_payload_exec_sig _initialAmount _tokenName _decimalUnits _tokenSymbol l).
+Defined.
+
+Lemma constructor_ls_payload_prf : forall (_initialAmount : ULValue uint256) 
+                                          (_tokenName : ULValue string) 
+                                          (_decimalUnits : ULValue uint8) 
+                                          (_tokenSymbol : ULValue string)
+                                          (l : LedgerLRecord rec) ,
+      constructor_ls_payload_exec _initialAmount _tokenName _decimalUnits _tokenSymbol l = 
+      exec_state (Uinterpreter (@constructor_ls_payload rec def _initialAmount _tokenName _decimalUnits _tokenSymbol)) l.
+Proof. 
+  intros.     
+  proof_of_2 constructor_ls_payload_exec constructor_ls_payload_exec_sig (constructor_ls_payload_exec_sig _initialAmount _tokenName _decimalUnits _tokenSymbol l).
+Qed.
+
+Tactic Notation "lift_all" "in" hyp(H) := (repeat  
+(rewrite exec_if_lift in H || 
+ rewrite eval_if_lift in H || 
+ rewrite toValue_if_lift in H )). 
+
+Opaque Common.hmapFindWithDefault
+       CommonInstances.addAdjustListPair
+       N.add N.sub N.leb N.ltb N.eqb Z.eqb N.pow.
+
+Definition constructor_ls_payload_exec_computed' (_initialAmount_value :  uint256)
+                                                 (_tokenName_value :  string)
+                                                 (_decimalUnits_value :  uint8)
+                                                 (_tokenSymbol_value :  string)
+                                                 (l: LedgerLRecord rec): True.  
+  assert (LedgerLRecord rec).
+  remember (local_left_field _ _ _ ("_initialAmount", 1%nat): ULValue uint256) as _initialAmount.
+  remember (local_left_field _ _ _ ("_tokenName", 1%nat): ULValue string) as _tokenName.
+  remember (local_left_field _ _ _ ("_decimalUnits", 1%nat): ULValue uint8) as _decimalUnits.
+  remember (local_left_field _ _ _ ("_tokenSymbol", 1%nat): ULValue string) as _tokenSymbol.
+  
+  remember (constructor_ls_pre_payload_computed _initialAmount_value _tokenName_value _decimalUnits_value _tokenSymbol_value l) as pre_exec.
+  remember (constructor_ls_payload_exec _initialAmount _tokenName _decimalUnits _tokenSymbol pre_exec) as exec.
+
+  destruct_ledger l.
+
+  time "constructor_ls_payload_exec unfold" unfold constructor_ls_payload_exec in Heqexec. 
+  time "constructor_ls_pre_payload_computed unfold" unfold constructor_ls_pre_payload_computed in Heqpre_exec.
+
+  unfold xBoolIfElse in Heqexec.
+  unfold boolFunRec in Heqexec. idtac.  
+  subst pre_exec _initialAmount _tokenName _decimalUnits _tokenSymbol. idtac.
+
+  time "lift" lift_all in Heqexec. idtac.
+  time "compute" compute in Heqexec. idtac.
+  time "buint" buint_all in Heqexec. idtac.
+   
+  (* symmetry in Heql1. idtac. *)     
+  match goal with
+  | Heql1: exec = ?LL |- _ => 
+    transparent_abstract exact_no_check LL using constructor_ls_payload_exec_computed_curried
+  end.
+  exact I.
+Defined.
+
+Check constructor_ls_payload_exec_computed_curried.
+About constructor_ls_payload_exec_computed_curried.
+(* mapping address uint256 ->
+       mapping address (mapping address uint256) ->
+       ContractLRecord ->
+       MessagesAndEventsLRecord ->
+       MessagesAndEventsLRecord ->
+       uint256 ->
+       uint256 ->
+       uint32 ->
+       uint64 ->
+       uint256 ->
+       address ->
+       uint128 ->
+       uint128 ->
+       address ->
+       cell_ ->
+       slice_ ->
+       boolean ->
+       uint128 ->
+       cell_ ->
+       boolean ->
+       boolean ->
+       Datatypes.list TracingTree -> uint32 -> rec *)
+
+
+Definition constructor_ls_payload_exec_computed
+                              (_initialAmount:  uint256)
+                              (_tokenName:  string)
+                              (_decimalUnits:  uint8)
+                              (_tokenSymbol:  string)
+                              (l: LedgerLRecord rec): LedgerLRecord rec.
+remember l as ledger. destruct_ledger l.
+refine (uncurry (f:=_GlobalClass) (constructor_ls_payload_exec_computed_curried _initialAmount _tokenName _decimalUnits _tokenSymbol)
+      (s, (s0, (* (s1, (s2, (s3, (s4, *)
+             (c0,
+              (m,
+               (m0,
+                (v0,
+                 (v1,
+                  (v2,
+                   (v3,
+                    (v4,
+                     (v5,
+                      (v6,
+                       (v7, (v8, (v9, (v10, (v11, (v12, (v13, (v14, (v15, (v16, (v17,
+                       l1)))))))))))))))))))))))%xprod).
+Defined.
+
+
+Lemma constructor_ls_payload_exec_computed_correct: forall (_initialAmount_value :  uint256)
+                                                           (_tokenName_value :  string)
+                                                           (_decimalUnits_value :  uint8)
+                                                           (_tokenSymbol_value :  string)
+                                                           (l: LedgerLRecord rec),
+  let _initialAmount := local_left_field _ _ _ ("_initialAmount", 1%nat) in
+  let _tokenName := local_left_field _ _ _ ("_tokenName", 1%nat) in
+  let _decimalUnits := local_left_field _ _ _ ("_decimalUnits", 1%nat) in
+  let _tokenSymbol := local_left_field _ _ _ ("_tokenSymbol", 1%nat) in  
+  let pre_exec := constructor_ls_pre_payload_computed _initialAmount_value _tokenName_value _decimalUnits_value _tokenSymbol_value l in
+      constructor_ls_payload_exec_computed _initialAmount_value _tokenName_value _decimalUnits_value _tokenSymbol_value l = 
+      constructor_ls_payload_exec _initialAmount _tokenName _decimalUnits _tokenSymbol pre_exec.
+Proof.
+  intros.
+  
+  remember (constructor_ls_payload_exec  _initialAmount _tokenName _decimalUnits _tokenSymbol pre_exec) as exec.
+  destruct_ledger l.  
+
+  time "constructor_ls_payload_exec unfold" unfold constructor_ls_payload_exec in Heqexec.
+  time "constructor_ls_pre_payload_computed unfold" unfold constructor_ls_pre_payload_computed in pre_exec.
+
+  unfold xBoolIfElse in Heqexec.
+  unfold boolFunRec in Heqexec. idtac.
+
+  unfold constructor_ls_pre_payload_computed in pre_exec.  
+  subst pre_exec _initialAmount _tokenName _decimalUnits _tokenSymbol. idtac.
+
+  time "lift" lift_all in Heqexec. idtac.
+  time "compute" compute in Heqexec. idtac.
+  time "buint" buint_all in Heqexec. idtac.
+  
+  auto.
+Qed. 
+
+
+Lemma constructor_exec_computed: forall
+                            (_initialAmount:  uint256)
+                            (_tokenName:  string)
+                            (_decimalUnits:  uint8)
+                            (_tokenSymbol:  string)
+                            (l: LedgerLRecord rec), 
+      exec_state (Uinterpreter (@constructor rec def _ _ _ _initialAmount _tokenName _decimalUnits _tokenSymbol))  
+                               {$$ l with Ledger_LocalState := default $$} =
+      constructor_ls_payload_exec_computed _initialAmount _tokenName _decimalUnits _tokenSymbol l. 
+Proof.
+  intros.
+  rewrite constructor_ls_template_exec_correct.
+  rewrite constructor_ls_payload_exec_computed_correct.
+  rewrite constructor_ls_payload_prf.
+
+  rewrite <- (constructor_ls_template_by_payload _initialAmount _tokenName _decimalUnits
+     _tokenSymbol l).
+
+  (* pose proof (constructor_ls_template_by_payload _initialAmount _tokenName _decimalUnits
+     _tokenSymbol l).
+  cbv zeta in H. rewrite <- H.   
+  rewrite <- constructor_ls_template_by_payload. *)
+
+  rewrite constructor_ls_template_exec_prf.
+  reflexivity.
+Qed.
+
 
